cfrontend/Cminorgenproof.v
@@ -1643,29 +1643,78 @@ Qed.
 
 (** Properties of [switch] compilation *)
 
-Remark switch_table_shift:
-  forall n sl base dfl,
-  switch_target n (S dfl) (switch_table sl (S base)) =
-  S (switch_target n dfl (switch_table sl base)).
+Inductive lbl_stmt_tail: lbl_stmt -> nat -> lbl_stmt -> Prop :=
+  | lstail_O: forall sl,
+      lbl_stmt_tail sl O sl
+  | lstail_S: forall c s sl n sl',
+      lbl_stmt_tail sl n sl' ->
+      lbl_stmt_tail (LScons c s sl) (S n) sl'.
+
+Lemma switch_table_default:
+  forall sl base,
+  exists n, 
+     lbl_stmt_tail sl n (select_switch_default sl)
+  /\ snd (switch_table sl base) = (n + base)%nat.
 Proof.
-  induction sl; intros; simpl. auto. destruct (Int.eq n i); auto. 
+  induction sl; simpl; intros.
+- exists O; split. constructor. omega.
+- destruct o. 
+  + destruct (IHsl (S base)) as (n & P & Q). exists (S n); split. 
+    constructor; auto. 
+    destruct (switch_table sl (S base)) as [tbl dfl]; simpl in *. omega.
+  + exists O; split. constructor. 
+    destruct (switch_table sl (S base)) as [tbl dfl]; simpl in *. auto.
 Qed.
 
-Remark length_switch_table:
-  forall sl base1 base2,
-  length (switch_table sl base1) = length (switch_table sl base2).
+Lemma switch_table_case:
+  forall i sl base dfl,
+  match select_switch_case i sl with
+  | None =>
+      switch_target i dfl (fst (switch_table sl base)) = dfl
+  | Some sl' =>
+      exists n,
+         lbl_stmt_tail sl n sl'
+      /\ switch_target i dfl (fst (switch_table sl base)) = (n + base)%nat
+  end.
 Proof.
-  induction sl; intros; simpl. auto. decEq; auto.
+  induction sl; simpl; intros.
+- auto.
+- destruct (switch_table sl (S base)) as [tbl1 dfl1] eqn:ST. 
+  destruct o; simpl.
+  rewrite Int.eq_sym. destruct (Int.eq i i0). 
+  exists O; split; auto. constructor.
+  specialize (IHsl (S base) dfl). rewrite ST in IHsl. simpl in *.
+  destruct (select_switch_case i sl).
+  destruct IHsl as (n & P & Q). exists (S n); split. constructor; auto. omega. 
+  auto.
+  specialize (IHsl (S base) dfl). rewrite ST in IHsl. simpl in *.
+  destruct (select_switch_case i sl).
+  destruct IHsl as (n & P & Q). exists (S n); split. constructor; auto. omega. 
+  auto.
+Qed.
+
+Lemma switch_table_select:
+  forall i sl,
+  lbl_stmt_tail sl
+                (switch_target i (snd (switch_table sl O)) (fst (switch_table sl O)))
+                (select_switch i sl).
+Proof.
+  unfold select_switch; intros.
+  generalize (switch_table_case i sl O (snd (switch_table sl O))). 
+  destruct (select_switch_case i sl) as [sl'|].
+  intros (n & P & Q). replace (n + O)%nat with n in Q by omega. congruence.
+  intros E; rewrite E.
+  destruct (switch_table_default sl O) as (n & P & Q).
+  replace (n + O)%nat with n in Q by omega. congruence.
 Qed.
 
 Inductive transl_lblstmt_cont(cenv: compilenv) (xenv: exit_env): lbl_stmt -> cont -> cont -> Prop :=
-  | tlsc_default: forall s k ts,
-      transl_stmt cenv (switch_env (LSdefault s) xenv) s = OK ts ->
-      transl_lblstmt_cont cenv xenv (LSdefault s) k (Kblock (Kseq ts k))
+  | tlsc_default: forall k,
+      transl_lblstmt_cont cenv xenv LSnil k (Kblock (Kseq Sskip k))
   | tlsc_case: forall i s ls k ts k',
-      transl_stmt cenv (switch_env (LScase i s ls) xenv) s = OK ts ->
+      transl_stmt cenv (switch_env (LScons i s ls) xenv) s = OK ts ->
       transl_lblstmt_cont cenv xenv ls k k' ->
-      transl_lblstmt_cont cenv xenv (LScase i s ls) k (Kblock (Kseq ts k')).
+      transl_lblstmt_cont cenv xenv (LScons i s ls) k (Kblock (Kseq ts k')).
 
 Lemma switch_descent:
   forall cenv xenv k ls body s,
@@ -1676,10 +1725,10 @@ Lemma switch_descent:
       plus step tge (State f s k sp e m) E0 (State f body k' sp e m)).
 Proof.
   induction ls; intros. 
-  monadInv H. econstructor; split.
-  econstructor; eauto.
-  intros. eapply plus_left. constructor. apply star_one. constructor. traceEq.
-  monadInv H. exploit IHls; eauto. intros [k' [A B]]. 
+- monadInv H. econstructor; split.
+  econstructor.
+  intros. eapply plus_two. constructor. constructor. auto. 
+- monadInv H. exploit IHls; eauto. intros [k' [A B]]. 
   econstructor; split.
   econstructor; eauto.
   intros. eapply plus_star_trans. eauto. 
@@ -1688,27 +1737,21 @@ Proof.
 Qed.
 
 Lemma switch_ascent:
-  forall f n sp e m cenv xenv k ls k1,
-  let tbl := switch_table ls O in
-  let ls' := select_switch n ls in
+  forall f sp e m cenv xenv ls n ls',
+  lbl_stmt_tail ls n ls' ->
+  forall k k1,
   transl_lblstmt_cont cenv xenv ls k k1 ->
   exists k2,
-  star step tge (State f (Sexit (switch_target n (length tbl) tbl)) k1 sp e m)
+  star step tge (State f (Sexit n) k1 sp e m)
              E0 (State f (Sexit O) k2 sp e m)
   /\ transl_lblstmt_cont cenv xenv ls' k k2.
 Proof.
-  induction ls; intros; unfold tbl, ls'; simpl.
-  inv H. econstructor; split. apply star_refl. econstructor; eauto.
-  simpl in H. inv H. 
-  rewrite Int.eq_sym. destruct (Int.eq i n).
-  econstructor; split. apply star_refl. econstructor; eauto. 
-  exploit IHls; eauto. intros [k2 [A B]].
-  rewrite (length_switch_table ls 1%nat 0%nat). 
-  rewrite switch_table_shift.
-  econstructor; split. 
-  eapply star_left. constructor. eapply star_left. constructor. eexact A. 
-  reflexivity. traceEq.
-  exact B.
+  induction 1; intros. 
+- exists k1; split; auto. apply star_refl.
+- inv H0. exploit IHlbl_stmt_tail; eauto. intros (k2 & P & Q). 
+  exists k2; split; auto.
+  eapply star_left. constructor. eapply star_left. constructor. eexact P.
+  eauto. auto. 
 Qed.
 
 Lemma switch_match_cont:
@@ -1720,22 +1763,6 @@ Proof.
   induction ls; intros; simpl.
   inv H0. apply match_Kblock2. econstructor; eauto.
   inv H0. apply match_Kblock2. eapply match_Kseq2. auto. eauto. 
-Qed.
-
-Lemma transl_lblstmt_suffix:
-  forall n cenv xenv ls body ts,
-  transl_lblstmt cenv (switch_env ls xenv) ls body = OK ts ->
-  let ls' := select_switch n ls in
-  exists body', exists ts',
-  transl_lblstmt cenv (switch_env ls' xenv) ls' body' = OK ts'.
-Proof.
-  induction ls; simpl; intros. 
-  monadInv H.
-  exists body; econstructor. rewrite EQ; eauto. simpl. reflexivity.
-  monadInv H.
-  destruct (Int.eq i n).
-  exists body; econstructor. simpl. rewrite EQ; simpl. rewrite EQ0; simpl. reflexivity.
-  eauto.
 Qed.
 
 Lemma switch_match_states:
@@ -1752,14 +1779,22 @@ Lemma switch_match_states:
   plus step tge (State tfn (Sexit O) tk' (Vptr sp Int.zero) te tm) E0 S
   /\ match_states (Csharpminor.State fn (seq_of_lbl_stmt ls) k e le m) S.
 Proof.
-  intros. destruct ls; simpl.
-  inv TK. econstructor; split. 
-    eapply plus_left. constructor. apply star_one. constructor. traceEq.
-    eapply match_state; eauto. 
-  inv TK. econstructor; split.
-    eapply plus_left. constructor. apply star_one. constructor. traceEq.
-    eapply match_state_seq; eauto.
-    simpl. eapply switch_match_cont; eauto.
+  intros. inv TK. 
+- econstructor; split. eapply plus_two. constructor. constructor. auto. 
+  eapply match_state; eauto. 
+- econstructor; split. eapply plus_left. constructor. apply star_one. constructor. auto.
+  simpl. eapply match_state_seq; eauto. simpl. eapply switch_match_cont; eauto.
+Qed.
+
+Lemma transl_lblstmt_suffix:
+  forall cenv xenv ls n ls',
+  lbl_stmt_tail ls n ls' ->
+  forall body ts, transl_lblstmt cenv (switch_env ls xenv) ls body = OK ts ->
+  exists body', exists ts', transl_lblstmt cenv (switch_env ls' xenv) ls' body' = OK ts'.
+Proof.
+  induction 1; intros. 
+- exists body, ts; auto.
+- monadInv H0. eauto. 
 Qed.
 
 (** Commutation between [find_label] and compilation *)
@@ -1778,10 +1813,9 @@ Lemma transl_lblstmt_find_label_context:
   find_label lbl ts tk1 = Some (ts', tk').
 Proof.
   induction ls; intros.
-  monadInv H. inv H0. simpl. simpl in H2. replace x with ts by congruence. rewrite H1. auto.
-  monadInv H. inv H0.
-  eapply IHls. eauto. eauto. simpl in H6. replace x with ts0 by congruence. simpl.
-  rewrite H1. auto.
+- monadInv H. inv H0. simpl. rewrite H1. auto.
+- monadInv H. inv H0. simpl in H6. eapply IHls; eauto. 
+  replace x with ts0 by congruence. simpl. rewrite H1. auto.
 Qed.
 
 Lemma transl_find_label:
@@ -1830,6 +1864,7 @@ Proof.
   (* block *)
   apply transl_find_label with (true :: xenv). auto. constructor; auto. 
   (* switch *)
+  simpl in H. destruct (switch_table l O) as [tbl dfl]. monadInv H. 
   exploit switch_descent; eauto. intros [k' [A B]].
   eapply transl_lblstmt_find_label. eauto. eauto. eauto. reflexivity.  
   (* return *)
@@ -1840,10 +1875,9 @@ Proof.
   apply transl_find_label with xenv; auto.
 
   intros. destruct ls; monadInv H; simpl.
-  (* default *)
-  inv H1. simpl in H3. replace x with ts by congruence. rewrite H2.
-  eapply transl_find_label; eauto.
-  (* case *)
+  (* nil *)
+  inv H1. rewrite H2. auto.
+  (* cons *)
   inv H1. simpl in H7.
   exploit (transl_find_label s). eauto. eapply switch_match_cont; eauto. 
   destruct (Csharpminor.find_label lbl s (Csharpminor.Kseq (seq_of_lbl_stmt ls) k)) as [[s' k''] | ].
@@ -1851,8 +1885,7 @@ Proof.
   exists ts'; exists tk'; exists xenv'; intuition. 
   eapply transl_lblstmt_find_label_context; eauto. 
   simpl. replace x with ts0 by congruence. rewrite H2. auto.
-  intro.
-  eapply transl_lblstmt_find_label. eauto. auto. eauto. 
+  intro. eapply transl_lblstmt_find_label. eauto. auto. eauto. 
   simpl. replace x with ts0 by congruence. rewrite H2. auto. 
 Qed.
 
@@ -2056,14 +2089,16 @@ Opaque PTree.set.
   eapply plus_left. constructor. apply plus_star; eauto. traceEq.
 
 (* switch *)
-  monadInv TR. left.
+  simpl in TR. destruct (switch_table cases O) as [tbl dfl] eqn:STBL. monadInv TR.
   exploit transl_expr_correct; eauto. intros [tv [EVAL VINJ]].
   inv VINJ.
   exploit switch_descent; eauto. intros [k1 [A B]].
-  exploit switch_ascent; eauto. intros [k2 [C D]].
-  exploit transl_lblstmt_suffix; eauto. simpl. intros [body' [ts' E]].
+  exploit switch_ascent; eauto. eapply (switch_table_select n).
+  rewrite STBL; simpl. intros [k2 [C D]].
+  exploit transl_lblstmt_suffix; eauto. eapply (switch_table_select n).
+  simpl. intros [body' [ts' E]].
   exploit switch_match_states; eauto. intros [T2 [F G]].
-  exists T2; split.
+  left; exists T2; split.
   eapply plus_star_trans. eapply B.  
   eapply star_left. econstructor; eauto. 
   eapply star_trans. eexact C. 
